examples/ghc/theories/Var.v
@@ -1,7 +1,27 @@
 Require Import Id.
 Require Import Core. (* For [Var] only *)
+Require Import Unique.
 
-(** ** Stuff about [Var] and [Id] *)
+Require Import Coq.Structures.Equalities.
+
+Require Import GHC.Base.
+Import GHC.Base.ManualNotations.
+
+Require Import Proofs.GHC.Base.
+
+Require Import Proofs.Unique.
+
+Ltac unfold_zeze :=
+  unfold GHC.Base.op_zeze__, Core.Eq___Var, op_zeze____, 
+  Core.Eq___Var_op_zeze__;
+  unfold GHC.Base.op_zeze__, Nat.Eq_nat, op_zeze____.  
+Ltac unfold_zsze :=
+  unfold GHC.Base.op_zsze__, Core.Eq___Var, op_zsze____, 
+  Core.Eq___Var_op_zsze__;
+  unfold GHC.Base.op_zsze__, Nat.Eq_nat, op_zsze____.  
+
+
+(** ** Stuff about [Var] and [Unique] *)
 
 Lemma getUnique_varUnique: 
     (Unique.getUnique : Var -> Unique.Unique) = varUnique.
@@ -11,6 +31,140 @@ Proof.
   auto.
 Qed.
 
+
+(** ** Properties about [GHC.Base.==] for Var. *)
+
+(* Equal vars have equal keys *)
+Lemma eq_unique : forall (v1 v2: Var), 
+    (v1 GHC.Base.== v2) = true <->
+    Unique.getWordKey (Unique.getUnique v1) = 
+    Unique.getWordKey (Unique.getUnique v2). 
+Proof.
+  intros v1 v2.
+  unfold_zeze.
+  unfold Unique.getUnique.
+  unfold Uniquable__Var, getUnique__, Core.Uniquable__Var_getUnique, 
+  varUnique.
+  destruct v1; destruct v2; simpl;
+  rewrite Nat2N.inj_iff;
+  apply Nat.eqb_eq.
+Qed.
+
+Instance EqLaws_Var : EqLaws Var := {}.
+Proof.
+  - unfold ssrbool.reflexive.
+    unfold_zeze.
+    intros. unfold is_true.
+    apply Nat.eqb_refl.
+  - unfold ssrbool.symmetric.
+    intros. unfold_zeze.
+    rewrite Nat.eqb_sym; auto.
+  - unfold ssrbool.transitive.
+    unfold_zeze.
+    unfold is_true.
+    intros x y z. 
+    destruct x; destruct y; destruct z; simpl;
+    repeat erewrite Nat.eqb_eq; intro h; rewrite h; auto.
+  - intros.
+    unfold_zsze.
+    unfold_zeze.
+    unfold negb.
+    destruct (realUnique x =? realUnique y); auto.
+Qed.    
+
+(** ** A DecidableType structure based on  [GHC.Base.==]. *)
+
+(* Define the Var type as a decidable type by using the Eq instance.
+   (This instance only looks at the Unique components of the Var *)
+
+Module Var_as_DT <: BooleanDecidableType <: DecidableType.
+  Definition t := Var.
+
+  Definition eqb : t -> t -> bool := _GHC.Base.==_.
+
+  Definition eq : t -> t -> Prop := fun x y => eqb x y = true.
+
+  Definition eq_equiv : Equivalence eq.
+  split. 
+  - unfold eq, eqb, Reflexive.
+    apply Eq_refl.
+  - unfold eq, eqb, Symmetric.
+    eauto using Eq_sym.
+  - unfold eq, eqb, Transitive.
+    intros x y z h1 h2.
+    eapply  Eq_trans; eauto.
+  Defined.
+
+  Definition eq_dec : forall x y : t, { eq x y } + { ~ (eq x y) }.
+  intros x y.
+  unfold eq, eqb.
+  unfold_zeze.
+  destruct x eqn:X; destruct y eqn:Y;  simpl.
+  all: destruct (Nat.eqb n0 n2) eqn:EQ ; [left; auto | right; auto].
+  Defined.
+
+  Lemma eqb_eq : forall x y, eqb x y = true <-> eq x y.
+    unfold eq. tauto.
+  Qed. 
+
+ Definition eq_refl := eq_equiv.(@Equivalence_Reflexive _ _).
+ Definition eq_sym := eq_equiv.(@Equivalence_Symmetric _ _).
+ Definition eq_trans := eq_equiv.(@Equivalence_Transitive _ _).
+
+End Var_as_DT.
+
+
+(** ** [almostEqual] *)
+
+(* Two [Var]s are almostEqual if they differ only in 
+   their IdInfo. All other components must be identitical.
+
+   We define this as a [Prop] rather than a bool because
+   we do not have a function that determines structural
+   equality.
+*)
+
+Inductive almostEqual : Var -> Var -> Prop :=
+ | AE_TyVar   : forall n u ty,
+   almostEqual (Mk_TyVar n u ty)
+               (Mk_TyVar n u ty)
+ | AE_TcTyVar : forall n u ty1 ty2,
+   almostEqual (Mk_TcTyVar n u ty1 ty2)
+               (Mk_TcTyVar n u ty1 ty2)
+ | AE_Id : forall n u ty ids idd id1 id2,
+   almostEqual (Mk_Id n u ty ids idd id1)
+               (Mk_Id n u ty ids idd id2).
+
+
+Lemma almostEqual_refl:
+  forall v, almostEqual v v.
+Proof. intros. destruct v; constructor. Qed.
+
+Lemma almostEqual_sym:
+  forall v1 v2,
+    almostEqual v1 v2 -> almostEqual v2 v1.
+Proof.
+  intros v1 v2 H.
+  inversion H; subst; eauto.
+  econstructor.
+Qed.
+
+Lemma almostEqual_trans:
+  forall v1 v2 v3, 
+    almostEqual v1 v2 -> almostEqual v2 v3 -> almostEqual v1 v3.
+Proof.
+  intros v1 v2 v3 H1 H2. 
+  inversion H1; inversion H2; subst; inversion H3; eauto.
+  econstructor.
+Qed.
+
+Lemma almostEqual_eq :
+  forall v1 v2, 
+    almostEqual v1 v2 -> (v1 GHC.Base.== v2 = true).
+Proof.
+  intros v1 v2 H.
+  inversion H; unfold_zeze; simpl; apply Nat.eqb_refl.
+Qed.
 
 (** ** [isJoinId] etc. *)
 
